# Shortest distance problems

```{index} Shortest distance
```

(shortest-distance-problems)=

We can take advantage of vector geometry to calculate the solutions to shortest distance problems.

---

(shortest-distance-between-two-points)=

```{index} Shortest distance ; point to point
```

## Shortest distance between two points

In $\mathbb{R}^n$ the shortest distance, $d$, between two points with position vectors $\mathbf{p}=(p_1, p_2, \ldots, p_n)$ and $\mathbf{q} = (q_1, q_2, \ldots, q_n)$ is the length of a straight line segment connecting them. If we think about this segment as of a vector, then

$$ d = \|\mathbf{p} - \mathbf{q}\| = \sqrt{\displaystyle\sum_{i=1}^n (p_i-q_i)^2}. $$

Note that $\|\mathbf{p} - \mathbf{q}\| = \|\mathbf{q} - \mathbf{p}\|$.

---

```{index} Shortest distance ; point to line
```

## Shortest distance between a line and a point

To the shortest distance, $d$, between a line $\mathbf{r} = \mathbf{p} + t\mathbf{d}$ and a point with position vector $\mathbf{q}$ in $\mathbb{R}^n$ is the length of the vector $\mathbf{q} - \mathbf{r}$ which is perpendicular to $\mathbf{d}$ ({numref}`line-point-distance-figure`).

```{figure} ../_images/4_line_point_distance.svg
:name: line-point-distance-figure
:width: 425

The shortest distance of a point $\mathbf{q}$ from the line $\mathbf{r} = \mathbf{p} + t \mathbf{d}$ is the length of the vector $\mathbf{q} - \mathbf{r}$ which is perpendicular to $\mathbf{d}$.
```

Since $\mathbf{q} - \mathbf{r}$ is perpendicular to $\mathbf{d}$ then since the dot product between two perpendicular vectors is zero then

$$ \mathbf{d} \cdot (\mathbf{r} - \mathbf{q}) = 0, $$

Substituting the {prf:ref}`vector equation of a line<vector-equation-of-a-line-definition>` and rearranging to make $t$ the subject gives

$$ \begin{align*}
    \mathbf{d} \cdot (\mathbf{r} - \mathbf{q}) &= 0 \\
    \mathbf{d} \cdot (\mathbf{p} + t \mathbf{d} - \mathbf{q}) &= 0 \\
    \mathbf{d} \cdot \mathbf{p} + t \mathbf{d} \cdot \mathbf{d} - \mathbf{d} \cdot \mathbf{q} &= 0 \\
    t \mathbf{d} \cdot \mathbf{d} &= (\mathbf{q} - \mathbf{p}) \cdot \mathbf{d} \\
    \therefore t &= \frac{(\mathbf{q} - \mathbf{p}) \cdot \mathbf{d}}{\mathbf{d} \cdot \mathbf{d}}.
\end{align*} $$

This gives the value of the parameter $t$ that can be used to calculate the position vector $\mathbf{r}$ and therefore the shortest distance between the point $\mathbf{q}$ and the line is $\|\mathbf{q} - \mathbf{r}\|$[^1].

[^1]: The dot product of between vector $\mathbf{a}$ and itself is sometimes denoted as $\mathbf{a}^2 = \mathbf{a} \cdot \mathbf{a}$.

```{prf:theorem} The shortest distance between a point and a line
:label: point-line-distance-theorem

The shortest distance between the point with position vector $\mathbf{q}$ and a line that passes through the point with position vector $\mathbf{p}$ in the direction $\mathbf{d}$ is $\|\mathbf{q} - \mathbf{r}\|$ where $\mathbf{r} = \mathbf{p} + t \mathbf{d}$ and

$$ t = \frac{(\mathbf{q} - \mathbf{p}) \cdot \mathbf{d}}{\mathbf{d} \cdot \mathbf{d}}. $$(point-line-t-equation)
```

<iframe width="560" height="315" src="https://www.youtube.com/embed/4cj0TIBLM4M?si=5cknsM4ka4Xe1YHg" title="YouTube video player" frameborder="0" allow="accelerometer; autoplay; clipboard-write; encrypted-media; gyroscope; picture-in-picture; web-share" allowfullscreen></iframe>

```{prf:example}
:label: point-line-distance-example

Find the shortest distance between the point with position vector $\mathbf{q} = (2,2,2)$ and the line $(t,t-2, t+1)$.

---

**Solution**

Writing the line in the form $\mathbf{r} = \mathbf{p} + t \mathbf{d}$

$$ \mathbf{r} = \begin{pmatrix} 0 \\ -2 \\ 1 \end{pmatrix} + t
\begin{pmatrix} 1 \\ 1 \\ 1 \end{pmatrix}, $$

so the direction vector is $\mathbf{d} = (1, 1, 1)$. Using equation {eq}`point-line-t-equation`

$$ \begin{align*}
    t &= \frac{\mathbf{d} \cdot \mathbf{q} - \mathbf{d} \cdot \mathbf{p}}{\mathbf{d} \cdot \mathbf{d}} \\
    &= \frac{
        \begin{pmatrix} 1 \\ 1 \\ 1 \end{pmatrix} \cdot
        \begin{pmatrix} 2 \\ 2 \\ 2 \end{pmatrix} -
        \begin{pmatrix} 1 \\ 1 \\ 1 \end{pmatrix} \cdot
        \begin{pmatrix} 0 \\ -2 \\ 1 \end{pmatrix}}{
        \begin{pmatrix} 1 \\ 1 \\ 1 \end{pmatrix} \cdot
        \begin{pmatrix} 1 \\ 1 \\ 1 \end{pmatrix}} \\
    &= \frac{6 + 1}{3} = \frac{7}{3}.
\end{align*} $$

So the point on the line which is closest to $\mathbf{q}$ is

$$ \begin{align*}
    \mathbf{r} =
    \begin{pmatrix} 0 \\ -2 \\ 1 \end{pmatrix} + \frac{7}{3}
    \begin{pmatrix} 1 \\ 1 \\ 1 \end{pmatrix} =
    \begin{pmatrix} 7/3 \\ 1/3 \\ 10/3 \end{pmatrix},
\end{align*} $$

and the shortest distance is $\|\mathbf{q} - \mathbf{r}\|$ so

$$ \begin{align*}
    \mathbf{q} - \mathbf{r} &= \begin{pmatrix} 2 \\ 2 \\ 2 \end{pmatrix} -
    \begin{pmatrix} 7/3 \\ 1/3 \\ 10/3 \end{pmatrix} =
    \begin{pmatrix} - 1/3 \\ 5/3 \\ -4/3 \end{pmatrix}, \\
    \therefore d &= \sqrt{\left(-\frac{1}{3}\right)^2 + \left(\frac{5}{3}\right)^2 + \left( -\frac{4}{3}\right)^2} \\
    &= \sqrt{\frac{14}{3}} \approx 2.16.
\end{align*} $$
```

---

```{index} Shortest distance ; line to line
```

## Shortest distance between two lines

Given two lines $\ell_1$ and $\ell_2$ described by $\mathbf{r}_1 = \mathbf{p}_1 + t \mathbf{d}_1$ and $\mathbf{r}_2 =  \mathbf{p}_2 + t \mathbf{d}_2$ in $\mathbb{R}^n$ we have three situations to consider

- If the two lines intersect then obviously the shortest distance is obviously 0.
- If the two lines are parallel then any point on $\ell_1$ can gives the shortest distance between $\ell_1$ and $\ell_2$. Hence we simply choose a point on $\ell_2$ and apply method for {prf:ref}`finding the distance between a point and a line<point-line-distance-theorem>`.
- If the two lines are skew then the shortest distance is the distance of the chord that is perpendicular to both $\ell_1$ and $\ell_2$ ({numref}`line-line-distance-figure`).

```{figure} ../_images/4_line_line_distance.svg
:name: line-line-distance-figure
:width: 350

The shortest distance between skew lines is the distance of the chord which is perpendicular to both lines.
```

If $\mathbf{r}_1$ and $\mathbf{r}_2$ are points on the lines $\ell_1$ and $\ell_2$ respectively then the chord $\mathbf{r}_1 \to  \mathbf{r}_2$ which is perpendicular to both lines has the direction vector $\mathbf{n} = \mathbf{d}_1 \times \mathbf{d}_2$. If $d$ is the distance between $\mathbf{r}_1$ and $\mathbf{r}_2$ then

$$ \mathbf{r}_2 - \mathbf{r}_1 = d \left( \frac{\mathbf{d}_1 \times \mathbf{d}_2}{\| \mathbf{d}_1 \times \mathbf{d}_2\|} \right), $$(line-line-distance-equation-1)

Let $\hat{\mathbf{n}} = \dfrac{\mathbf{d}_1 \times \mathbf{d}_2}{\|\mathbf{d}_1 \times \mathbf{d}_2\|}$ and substituting the equations of $\mathbf{r}_1$ and $\mathbf{r}_2$ equation {eq}`line-line-distance-equation-1` gives

$$ \begin{align*}
    \mathbf{r}_2 - \mathbf{r}_1 &= d \hat{\mathbf{n}}\\
    (\mathbf{p}_2 + t_2 \mathbf{d}_2) - (\mathbf{p}_1 + t_1 \mathbf{d}_1)
    &= d \hat{\mathbf{n}}\\
    (\mathbf{p}_2 + t_2 \mathbf{d}_2) \cdot \hat{\mathbf{n}} - (\mathbf{p}_1 + t_1 \mathbf{d}_1) \cdot \hat{\mathbf{n}}
    &= d \hat{\mathbf{n}} \cdot \hat{\mathbf{n}} \\
    \mathbf{p}_2 \cdot \hat{\mathbf{n}} + t_2 \mathbf{d}_2 \cdot \hat{\mathbf{n}} - \mathbf{p}_1 \cdot \hat{\mathbf{n}} - t_1 \mathbf{d}_1 \cdot \hat{\mathbf{n}}
    &= d \hat{\mathbf{n}} \cdot \hat{\mathbf{n}}.
\end{align*} $$

Since $\mathbf{n}$ is perpendicular to both $\ell_1$ and $\ell_2$ then $\mathbf{d}_1 \cdot \mathbf{n} = \mathbf{d}_2 \cdot \mathbf{n} = 0$ and $\hat{\mathbf{n}} \cdot \hat{\mathbf{n}} = 1$ then

$$ \mathbf{p}_2 \cdot \hat{\mathbf{n}} - \mathbf{p}_1 \cdot \hat{\mathbf{n}} = d, $$

which simplifies to

$$ d = (\mathbf{p}_2 - \mathbf{p}_1) \cdot \hat{\mathbf{n}}. $$

```{prf:theorem} The shortest distance between two skew lines
:label: line-line-distance-theorem

The shortest distance between two skew lines $\mathbf{r}_1 = \mathbf{p}_1 + t_1 \mathbf{d}_1$ and $\mathbf{r}_2 = \mathbf{p}_2 + t_2 \mathbf{d}_2$ is

$$ d = (\mathbf{p}_2 - \mathbf{p}_1) \cdot \hat{\mathbf{n}}.$$(line-line-distance-equation)

where $\hat{\mathbf{n}} = \dfrac{\mathbf{d}_1 \times \mathbf{d}_2}{\|\mathbf{d}_1 \times \mathbf{d}_2\|}$.
```

<iframe width="560" height="315" src="https://www.youtube.com/embed/4cj0TIBLM4M?si=-VjP5H3OCMDD_zOp&amp;start=304" title="YouTube video player" frameborder="0" allow="accelerometer; autoplay; clipboard-write; encrypted-media; gyroscope; picture-in-picture; web-share" allowfullscreen></iframe>

```{prf:example}
:label: line-line-distance-example

Find the shortest distance between the two skew lines $\ell_1$ and $\ell_2$ defined by $(t_1, 1 + 4t_1, 3 + 2 t_1)$ and $(1, 1 + 2t_2, 3 + 4t_2)$ respectively.

---

**Solution**

First, we need to identify the direction vectors $\mathbf{d}_1$ and $\mathbf{d}_2$. Writing $\ell_1$ and $\ell_2$ in the form $\mathbf{r} = \mathbf{p} + t \mathbf{d}$

$$ \begin{align*}
    \mathbf{r}_1 &= \mathbf{p}_1 + t_1 \mathbf{d}_1 = \begin{pmatrix} 0 \\ 1 \\ 3 \end{pmatrix} + t_1
    \begin{pmatrix} 1 \\ 4 \\ 2 \end{pmatrix} , \\
    \mathbf{r}_2 &= \mathbf{p}_2 + t_2 \mathbf{d}_2 = \begin{pmatrix} 1 \\ 1 \\ 3 \end{pmatrix} + t_2
    \begin{pmatrix} 0 \\ 2 \\ 4 \end{pmatrix},
\end{align*} $$

therefore $\mathbf{d}_1 = (1, 4, 2)$ and $\mathbf{d}_2 = (0, 2, 4)$. Now we can calculate $\hat{\mathbf{n}}$

$$ \begin{align*}
    \mathbf{n} &= \mathbf{d}_1 \times \mathbf{d}_2
    = \begin{vmatrix}
        \mathbf{i} & \mathbf{j} & \mathbf{k} \\
        1 & 4 & 2 \\
        0 & 2 & 4
    \end{vmatrix} =
    \begin{pmatrix} 12 \\ -4 \\ 2 \end{pmatrix}, \\
    \|\mathbf{n}\| &= \sqrt{12^2 + (-4)^2 + 2^2} = \sqrt{164} = 2\sqrt{41}, \\
    \therefore \hat{\mathbf{n}} &= \frac{\mathbf{n}}{\|\mathbf{n}\|}
    = \frac{1}{2\sqrt{41}}
    \begin{pmatrix} 12 \\ -4 \\ 2 \end{pmatrix}
    =
    \begin{pmatrix} 6\sqrt{41}/41 \\ -2\sqrt{41}/41 \\ \sqrt{41}/41 \end{pmatrix}.
\end{align*} $$

Note that since $\mathbf{n}$ is non-zero, $\ell_1$ and $\ell_2$ are skew lines. Using equation {eq}`line-line-distance-equation`

$$ \begin{align*}
    d &= (\mathbf{p}_2 - \mathbf{p}_1) \cdot \hat{\mathbf{n}} \\
    &= \left( \begin{pmatrix} 1 \\ 1 \\ 3 \end{pmatrix} -
    \begin{pmatrix} 0 \\ 1 \\ 3 \end{pmatrix} \right) \cdot
    \begin{pmatrix} 6\sqrt{41}/41 \\ -2\sqrt{41}/41 \\ \sqrt{41}/41 \end{pmatrix} \\
    &= \begin{pmatrix} 1 \\ 0 \\ 0 \end{pmatrix} \cdot
    \begin{pmatrix} 6\sqrt{41}/41 \\ -2\sqrt{41}/41 \\ \sqrt{41}/41 \end{pmatrix} \\
    &= \frac{6 \sqrt{41}}{41}.
\end{align*} $$
```
