(cramers-rule-section)=

```{index} Cramer's rule
```

```{index} Systems of linear equations ; solution using Cramer's rule
```

# Cramer's rule

```{figure} https://upload.wikimedia.org/wikipedia/commons/thumb/6/6d/Gabriel_Cramer.jpg/220px-Gabriel_Cramer.jpg
:width: 200
:alt: Gabriel Cramer
:figclass: margin

<a href="https://en.wikipedia.org/wiki/Gabriel_Cramer" target="_blank">Gabriel Cramer (1704 - 1752)</a>
```

**Cramer's rule**, named after Swiss mathematician <a href="https://en.wikipedia.org/wiki/Gabriel_Cramer" target="_blank">Gabriel Cramer</a>, is an explicit rule for calculating the solution to a system of linear equations using determinants. We saw in the section on [when systems are solvable](requirements-for-systems-of-linear-equations-to-be-solvable-section)) that the solution to the system of linear equations

$$ \begin{pmatrix} a & b \\ c & d \end{pmatrix}
    \begin{pmatrix} x_1 \\ x_2 \end{pmatrix} =
    \begin{pmatrix} e \\ f \end{pmatrix}$$

is

$$ \begin{align*}
    x_1 &= \frac{de - bf}{ad - bc}, & \qquad
    x_2 &= \frac{af - ce}{ad - bc}.
\end{align*} $$

The solution to both variables includes the determinant of the coefficient matrix, $ad - bc$, in the denominator. But what about the numerator? If we consider the value of $x_1$, which is $de - bf$, we can see that it includes the constant values $e$ and $f$, and we have the difference of two products - which is similar to the determinant of a $2 \times 2$ matrix. In fact, we can say which matrix this is the determinant of:

$$ \begin{align*}
    de - bf = \begin{vmatrix} e & b \\ f & d \end{vmatrix}.
\end{align*} $$

Performing a similar analysis for the solution to $x_2$, we see that the numerator is

$$ \begin{align*}
    af - ce = \begin{vmatrix} a & e \\ c & f \end{vmatrix}.
\end{align*} $$

These matrices are simply the coefficient matrix $\begin{pmatrix} a & b \\ c & d \end{pmatrix}$ with columns 1 and 2 replaced by the constant vector $\begin{pmatrix} e \\ f \end{pmatrix}$ for $x_1$ and $x_2$ respectively. This idea can be extended to larger systems, and is known as Cramer's rule.

````{prf:theorem} Cramer's rule
:label: cramers-rule-theorem

The solution to a non-singular linear system of equations of the form $A\mathbf{x}=\mathbf{b}$ can be calculated using Cramer's rule which is

$$ x_i = \frac{\det(A_i)}{\det(A)}, $$(cramers-rule-equation)

where $A_i$ is the matrix obtained by replacing column $i$ of $A$ with $\mathbf{b}$.
````

```{prf:proof}

The solution to a system of linear equations $A \mathbf{x} = \mathbf{b}$ can be calculated as $\mathbf{x} = A^{-1} \mathbf{b}$, where $A^{-1}$ is the inverse of the coefficient matrix $A$. The {prf:ref}`adjoint-determinant formula<adjoint-determinant-formula-theorem>` for calculating the inverse is

$$ A^{-1} = \frac{\operatorname{adj}(A)}{\det(A)}, $$

so

$$ \mathbf{x} = \frac{1}{\det(A)} \operatorname{adj}(A) \mathbf{b}. $$

Since $\operatorname{adj}(A) = C^\mathsf{T}$ where $C$ is the matrix of {prf:ref}`co-factors<cofactor-definition>`

$$ \operatorname{adj}(A) = C^\mathsf{T} = \begin{pmatrix}
    C_{11} & C_{21} & \cdots & C_{n1} \\
    C_{12} & C_{22} & \cdots & C_{n2} \\
    \vdots & \vdots & \ddots & \vdots \\
    C_{1n} & C_{2n} & \cdots & C_{nn}
\end{pmatrix}. $$

then for the $i$th element of $\mathbf{x}$, using the {prf:ref}`definition of matrix multiplication<matrix-multiplication-definition>` we have

$$ x_i = \frac{1}{\det(A)} \sum_{j=1}^n C_{ji} b_j $$

In Cramer's rule, $A_i$ is the matrix formed by replacing the $i$th column of $A$ with $\mathbf{b}$

$$ A_i = \begin{pmatrix}
        a_{11} & \cdots & a_{1,i-1} & b_1 & a_{1,i+1} & \cdots & a_{1n} \\
        a_{21} & \cdots & a_{2,i-1} & b_2 & a_{2,i+1} & \cdots & a_{2n} \\
        \vdots & \ddots & \vdots & \vdots & \vdots & \ddots & \vdots \\
        a_{n1} & \cdots & a_{n,i-1} & b_n & a_{n,i+1} & \cdots & a_{nn}
    \end{pmatrix}. $$

Since removing the $i$th column from both $A$ and $A_i$ (the one with the $b$ values) results in the same matrix then the cofactors of $A_i$ are the same as the cofactors of $A$. If we calculate $\det(A_i)$ by expanding along the $i$th column of $A_i$ then

$$ \det(A_i) = b_1 C_{1i} + b_2 C_{2i} + \cdots + b_n C_{ni} = \sum_{j=1}^n C_{ji} b_j, $$

so $x_i = \dfrac{\det(A_i)}{\det(A)}$.
```

<iframe width="560" height="315" src="https://www.youtube.com/embed/A4eghvWJwL0?si=TEHoBgFCx22xKWQK" title="YouTube video player" frameborder="0" allow="accelerometer; autoplay; clipboard-write; encrypted-media; gyroscope; picture-in-picture; web-share" allowfullscreen></iframe>

```{prf:example}
:label: cramers-rule-example

Solve the following systems of linear equations using Cramer's rule

(i) &emsp; $\begin{array}{rl}
    3x_1 - 2x_2  \!\!\!\! &= -4, \\
    x_1 - 3x_2  \!\!\!\! &= 1.
\end{array}$; &emsp;
(ii) &emsp; $\begin{array}{rl}
    -2x_1 - 3x_2 - x_3 \!\!\!\!  &= -5, \\
    -4x_1 + 4x_2 + 3x_3  \!\!\!\! &= -20, \\
    -3x_1  \!\!\!\! &= -12.
\end{array}$

```{dropdown} Solution

(i) &emsp; Here $A = \begin{pmatrix} 3 & -2 \\ 1 & -3 \end{pmatrix}$ and $\mathbf{b} = \begin{pmatrix} -4 \\ 1 \end{pmatrix}$

$$ \begin{align*}
    x_1 &= \frac{
    \begin{vmatrix} -4 & -2 \\ 1 & -3 \end{vmatrix}}
    {\begin{vmatrix} 3 & -2 \\ 1 & -3 \end{vmatrix}} = \frac{14}{-7} = -2,  \\
    \\
    x_2 &= \frac{\begin{vmatrix} 3 & -4 \\ 1 & 1 \end{vmatrix}}{-7} =
    \frac{7}{-7} = -1.
\end{align*} $$

Checking the solution

$$ \begin{align*}
    A\mathbf{x} = \begin{pmatrix} 3 & -2 \\ 1 & -3 \end{pmatrix}
    \begin{pmatrix} -2 \\ -1 \end{pmatrix} =
    \begin{pmatrix} -4 \\ 1 \end{pmatrix} = \mathbf{b} \qquad \checkmark
\end{align*} $$

(ii) &emsp; Here $A = \begin{pmatrix} -2 & -3 & -1 \\ -4 & 4 & 3 \\ -3 & 0 & 0 \end{pmatrix}$ and $\mathbf{b} = \begin{pmatrix} -5 \\ -20 \\ -12 \end{pmatrix}$

$$ \begin{align*}
    x_1 &= \frac{
    \begin{vmatrix}-5 & -3 & -1 \\ -20 & 4 & 3 \\ -12 & 0 & 0 \end{vmatrix}}
    {\begin{vmatrix} -2 & -3 & -1 \\ -4 & 4 & 3 \\ -3 & 0 & 0 \end{vmatrix}}
    = \frac{-12
    \begin{vmatrix} -3 & -1 \\ 4 & 3 \end{vmatrix}}
    {-3\begin{vmatrix} -3 & -1 \\ 4 & 3 \end{vmatrix}}
    = \frac{-12 \cdot -5}{-3 \cdot -5} = \frac{60}{15} = 4,\\ \\
    x_2 &= \frac{
    \begin{vmatrix} -2 & -5 & -1 \\ -4 & -20 & 3 \\ -3 & -12 & 0 \end{vmatrix}}{15}
    = \frac{-\begin{vmatrix} -4 & -20 \\ -3 & -12 \end{vmatrix}
    - 3\begin{vmatrix}-2 & -5 \\ -3 & -12 \end{vmatrix}}{15}
    = \frac{12 - 3 \cdot 9}{15} = \frac{-15}{15} = -1, \\ \\
    x_3 &= \frac{
    \begin{vmatrix} -2 & -3 & - 5 \\ -4 & 4 & -20 \\ -3 & 0 & -12 \end{vmatrix}}{15}
    =\frac{-3\begin{vmatrix} -3 & -5 \\ 4 & -20 \end{vmatrix} -
    12\begin{vmatrix} -2 & -3 \\ -4 & 4 \end{vmatrix}}{15}
     = \frac{-3 \cdot 80 - 12 \cdot -20}{15} = \frac{0}{15} = 0.
\end{align*} $$

Checking the solution

$$ \begin{align*}
    A\mathbf{x} =
    \begin{pmatrix} -2 & -3 & -1 \\ -4 & 4 & 3 \\ -3 & 0 & 0 \end{pmatrix}
    \begin{pmatrix} 4 \\ -1 \\ 0 \end{pmatrix} =
    \begin{pmatrix} -5 \\ -20 \\ -12 \end{pmatrix} = \mathbf{b} \qquad \checkmark
\end{align*} $$
```
