(linear-transformations-chapter)=

```{index} Linear transformations
```

# Linear Transformations

You will already be familiar with the use of <a href="https://en.wikipedia.org/wiki/Function_(mathematics)" target="_blank">functions</a> in mathematics to study sets and the **mapping** from a set of inputs set to another set of outputs. The notation used to denote functions is of the form $f: X \to Y$ where $f$ is the name of the function, $X$ is the set of inputs known as the **domain** and $Y$ is a member of the set of outputs known as the **co-domain**. The mapping which defines the relationship between the domain and co-domain is defined using $y = f(x)$ where $x$ is a member of the domain and $y$ is a member of the co-domain.

In linear algebra we study the linear mapping of a set of vectors to another set of vectors, so we define $T: V \to W$ where $V$ and $W$ are vector spaces and the mapping from an input vector $\mathbf{u} \in V$ to an output vector $\mathbf{w} \in W$ is given by $\mathbf{w} = T(\mathbf{u})$.

Linear transformations have lots of uses in mathematics and computing. A good example is in the field of computer graphics and computer games where they are fundamental to the manipulation and visualisation of three-dimensional objects.

We begin with the formal definition of a linear transformation.

```{prf:definition} Linear transformation
:label: linear-transformation-definition

If $V$ and $W$ are two vector spaces over the same field $F$ then by a **linear transformation** (or **linear mapping**) is a mapping $T: V \to W$ that for any two vectors $\mathbf{u}, \mathbf{v} \in V$ and any scalar $\alpha \in F$ the following conditions hold

- addition operation: $T(\mathbf{u} + \mathbf{v}) = T(\mathbf{u}) + T(\mathbf{v})$;
- scalar multiplication:  $T(\alpha \mathbf{u}) = \alpha T(\mathbf{u})$.

The result of applying a linear transformation to an object is known as the **image**.
```

For example, let $V = \mathbb{R}^2$ and $W = \mathbb{R}^3$ then $T : V \to W$ defined by $T : (x, y) \mapsto (x, y, 0)$ is a linear transformation. Let $\mathbf{u} = (u_1, u_2), \mathbf{v} = (v_1, v_2) \in \mathbb{R}^2$ and $\alpha \in \mathbb{R}$ then

$$ \begin{align*}
    T (\mathbf{u} + \mathbf{v})
    &= T \begin{pmatrix} u_1 + v_1 \\ u_2 + v_2 \end{pmatrix}
    = \begin{pmatrix} u_1 + v_1 \\ u_2 + v_2 \\ 0 \end{pmatrix}, \\
    T (\mathbf{u}) + T(\mathbf{v}) &=
    \begin{pmatrix} u_1 \\ u_2 \\ 0 \end{pmatrix} + \begin{pmatrix} v_1 \\ v_2 \\ 0 \end{pmatrix}
    = \begin{pmatrix} u_1 + v_1 \\ u_2 + v_2 \\ 0 \end{pmatrix},
\end{align*} $$

so $T(\mathbf{u} + \mathbf{v}) = T(\mathbf{u}) + T(\mathbf{v})$ and the addition condition is satisfied. Similarly

$$ \begin{align*}
    T(\alpha \mathbf{u})
    &= T \begin{pmatrix} \alpha u_1 \\ \alpha u_2 \end{pmatrix}
    = \begin{pmatrix} \alpha u_1 \\ \alpha u_2 \\ 0 \end{pmatrix}, \\
    \alpha T(\mathbf{u}) &= \alpha \begin{pmatrix} u_1 \\ u_2 \\ 0 \end{pmatrix}
    = \begin{pmatrix} \alpha u_1 \\ \alpha u_2 \\ 0 \end{pmatrix},
\end{align*} $$

so $T(\alpha \mathbf{u}) = \alpha T(\mathbf{u})$ and the scalar multiplication condition is satisfied and combined with the addition condition we have shown that $T$ is a linear transformation. We can combine the addition and scalar multiplication conditions to give a single condition.

```{prf:definition} Linear transformation condition
:label: linear-transformation-condition -definition

A transformation $T : V \to W$ is a linear transformation if the following condition is satisfied for any $\mathbf{u}, \mathbf{v} \in V$ and $\alpha \in F$

$$ T(\mathbf{u} + \alpha \mathbf{v}) = T(\mathbf{u}) + \alpha T(\mathbf{v}). $$(linear-transformation-condition-equation)
```

```{prf:example}
:label: linear-transformation-example

Determine which of the following transformations are linear transformations

(i) &emsp; $T: \mathbb{R}^3 \to \mathbb{R}^2$ defined by $T: (x, y, z) \mapsto (x, y)$

(ii) &emsp; $T: \mathbb{R}^3 \to \mathbb{R}^2$ defined by $T: (x, y, z) \mapsto (x + 3, y)$

(iii) &emsp; $T: P(\mathbb{R}) \to P(\mathbb{R})$ defined by $T: p \mapsto p \dfrac{\mathrm{d}p}{\mathrm{d}x}$

```{dropdown} Solution

(i) &emsp; Let $\mathbf{u} = (u_1, u_2, u_3), \mathbf{v} = (v_1, v_2, v_3) \in \mathbb{R}^3$ and $\alpha \in \mathbb{R}$ then

$$ \begin{align*}
    T(\mathbf{u} + \alpha \mathbf{v}) &= T\left(
        \begin{pmatrix} u_1 \\ u_2 \\ u_3 \end{pmatrix} + \alpha
        \begin{pmatrix} v_1 \\ v_2 \\ v_3 \end{pmatrix}
    \right)
    = T \begin{pmatrix} u_1 + \alpha v_1 \\ u_2 + \alpha v_2 \\ u_3 + \alpha v_3 \end{pmatrix}
    = \begin{pmatrix} u_1 + \alpha v_1 \\  u_2 + \alpha v_2 \end{pmatrix}, \\
    T(\mathbf{u}) + \alpha T(\mathbf{v}) &= T
    \begin{pmatrix} u_1 \\ u_2 \\ u_3 \end{pmatrix} + \alpha T
    \begin{pmatrix} v_1 \\ v_2 \\ v_3 \end{pmatrix} =
    \begin{pmatrix} u_1 \\ u_2 \end{pmatrix} + \alpha
    \begin{pmatrix} v_1 \\ v_2 \end{pmatrix} =
    \begin{pmatrix} u_1 + \alpha v_1 \\ u_2 + \alpha v_2 \end{pmatrix}.
\end{align*} $$

Since $T(\mathbf{u} + \alpha \mathbf{v}) = T(\mathbf{u}) + \alpha T(\mathbf{v})$ then $T: (x, y, z) \mapsto (x, y)$ is a linear transformation.

(ii) &emsp; Let $\mathbf{u} = (u_1, u_2, u_3), \mathbf{v} = (v_1, v_2, v_3) \in \mathbb{R}^3$ and $\alpha \in \mathbb{R}$ then

$$ \begin{align*}
    T(\mathbf{u} + \alpha \mathbf{v}) &= T
    \begin{pmatrix} u_1 + \alpha v_1 \\ u_2 + \alpha v_2 \\ u_3 + \alpha v_3 \end{pmatrix}
    = \begin{pmatrix} u_1 + \alpha v_1 + 3 \\ u_2 + \alpha v_2 \end{pmatrix}, \\
    T(\mathbf{u}) + \alpha T(\mathbf{v}) &= T
    \begin{pmatrix} u_1 \\ u_2 \\ u_3 \end{pmatrix} + \alpha T
    \begin{pmatrix} v_1 \\ v_2 \\ v_3 \end{pmatrix} =
    \begin{pmatrix} u_1 + 3 \\ u_2 \end{pmatrix} + \alpha
    \begin{pmatrix} v_1 + 3 \\ v_2 \end{pmatrix}
    =
    \begin{pmatrix} u_1 + v_1 + 3 + 3\alpha \\ u_2 + \alpha v_2 \end{pmatrix}
\end{align*} $$

Since $T(\mathbf{u} + \alpha \mathbf{v}) \neq T(\mathbf{u}) + \alpha T(\mathbf{v})$ then $T: (x, y, z) \mapsto (x + 3, y)$ is not a linear transformation.

Note that we could have shown this by a counterexample, e.g., let $\mathbf{u} = ( 1, 0 , 0 ), \mathbf{v} = (2, 0, 0) \in \mathbb{R}^3$ then

$$ \begin{align*}
    T(\mathbf{u} + \mathbf{v}) &= T
    \begin{pmatrix} 3 \\ 0 \\ 0 \end{pmatrix}
    = \begin{pmatrix} 6 \\ 0 \end{pmatrix}, \\
    T(\mathbf{u}) + T(\mathbf{v}) &=
    \begin{pmatrix} 4 \\ 0 \\ 0 \end{pmatrix} + \begin{pmatrix} 5 \\ 0 \\ 0 \end{pmatrix}
    = \begin{pmatrix} 9 \\ 0 \end{pmatrix}.
\end{align*} $$

(iii) &emsp; Let $u = x \in P(\mathbb{R})$ then

$$ \begin{align*}
    T(2u) &= T(2x) = 2x(2) = 4x, \\
    2T(u) &= 2T(x) = 2(x)(1) = 2x,
\end{align*}  $$

therefore $T(2u) \neq 2T(u)$ and $T: p \mapsto p \dfrac{\mathrm{d}p}{\mathrm{d}x}$ is not a linear transformation.
```

(transformation-matrix-section)=

```{index} Linear transformations ; transformation matrices
```
