(composite-linear-transformations-section)=

```{index} Linear transformations ; composite transformations
```

# Composite linear transformations

```{prf:definition} Composite transformations
:label: composite-transformation-definition

Let $T : V \to W$ and $S: W \to X$ be two linear transformations over the vector spaces $V, W$ and $X$. The **composition** of $S$ and $T$ is the transformation $S \circ T: V \to X$ defined by

$$ (S \circ T)(\mathbf{u}) = S(T(\mathbf{u})), $$

for all vectors $\mathbf{u} \in V$.
```

For example, let $T$ and $S$ be two linear transformations on $\mathbb{R}^3$, defined by $T:(x, y, z) \mapsto (2 x + 4 y, -x + 3 y, x + 2 y)$ and $S:(x, y, z) \mapsto (2x + y - z, 3x + z, y - 2z)$.

The composite linear transformation $S \circ T(x, y, z)$ is

$$ \begin{align*}
    S \circ T\begin{pmatrix} x \\ y \\ z \end{pmatrix} &=
    S \left( T\begin{pmatrix} x \\ y \\ z \end{pmatrix} \right)
    = S \begin{pmatrix} 2 x + 4 \\ - x + 3y \\ x + 2 y \end{pmatrix} \\
    &= \begin{pmatrix}
        2(2 x + 4 y) + (-x + 3 y) - (x + 2 y) \\
        3(2 x + 4 y) + (x + 2 y) \\
        (-x + 3 y) - 2(x + 2 y)
    \end{pmatrix} \\
    &= \begin{pmatrix} 2 x + 9 y \\ 7 x + 14 y \\ -3 x - y \end{pmatrix},
\end{align*} $$

i.e., $S \circ T(x,y , z) \mapsto (2x + 9y, 7x + 14y, -3x - y)$.

---

## Composite transformation matrices

We have seen that a linear transformation $T: V \to W$ can be represented by a {prf:ref}`transformation matrix<transformation-matrix-definition>`, so that given a vector $\mathbf{u} \in V$ the image is calculated as:

$$ T(\mathbf{u}) = A \mathbf{u}. $$(composite-transformation-matrix-equation-1)

Consider the composition of $T$ with another linear transformation $S: W \to X$, where $S$ has a transformation matrix $B$:

$$ S \circ T(\mathbf{u}) = B \cdot T(\mathbf{u}) $$(composite-transformation-matrix-equation-2)

Substituting equation {eq}`composite-transformation-matrix-equation-1` into equation {eq}`composite-transformation-matrix-equation-2` gives

$$ S \circ T (\mathbf{u}) = B \cdot A \mathbf{u}. $$

```{prf:theorem} Composite transformation matrices
:label: composite-transformation-matrices-theorem

Given two linear transformations $T:V \to W$ and $S:W \to X$ with transformation matrices $A$ and $B$ respectively, the image of the vector $\mathbf{u} under the composition $S \circ T$  \in V$ is:

$$ S \circ T (\mathbf{u}) = B \cdot A \cdot \mathbf{u}. $$(composite-transformation-matrices-theorem-equation)
```

Note that the matrices here occur in the same order as the functions are listed in the composition, which is the reverse of the order in which they are applied to the vector. Here, we apply the function $T$ first, then the function $S$, but they are written as $S$ first then $T$.

To apply the transformation, we can multiply the matrices together and then multiply this by the vector on the left - but note that we need to calculate $B \cdot A$, since the order of matrix multiplication matters. 

```{prf:example}
:label: composite-transformation-matrix-example

Write down the transformation matrices $A$ and $B$ for the transformations $T:(x, y, z) \mapsto (2 x + 4 y, -x + 3 y, x + 2 y)$ and $S:(x, y, z) \mapsto (2x + y - z, 3x + z, y - 2z)$ respectively. Use them to calculate the transformation matrix $C$ for $S\circ T$.

```{dropdown} Solution

The transformation matrices for $T$ and $S$ are:

$$ \begin{align*}
    A &= \begin{pmatrix} 2 & 4 \\ -1 & 3 \\ 1 & 2 \end{pmatrix}, &
    B &= \begin{pmatrix} 2 & 1 & - 1 \\ 3 & 0 & 1 \\ 0 & 1 & -2 \end{pmatrix}.
\end{align*} $$

The transformation matrix for the composite transformation $S \circ T$ is $C = BA$:

$$ \begin{align*}
    C &= BA = \begin{pmatrix} 2 & 1 & - 1 \\ 3 & 0 & 1 \\ 0 & 1 & -2 \end{pmatrix}
    \begin{pmatrix} 2 & 4 \\ -1 & 3 \\ 1 & 2 \end{pmatrix}
    = \begin{pmatrix} 2 & 9 \\ 7 & 14 \\ -3 & -1 \end{pmatrix}.
\end{align*} $$

So $S \circ T(x,y , z) \mapsto (2x + 9y, 7x + 14y, -3x - y)$, as we saw in the example above.
```
