(exam-2023)=

# Exam 2023

1\. Given the two matrices $A = \begin{pmatrix} 0 & -1 & 5 \\ 8 & 1 & 2 \\ 5 & 2 & -1 \end{pmatrix}$ and $\mathbf{b} = \begin{pmatrix} 2 \\ 1 \\ 0 \end{pmatrix}.$

(a) &emsp; Calculate the inverse of $A$ and show that your inverse is correct.

(b) &emsp; Calculate $\operatorname{rank}(A)$ and $\operatorname{rank}([A \mid \mathbf{b}])$ and hence determine if the system $A \mathbf{x} = \mathbf{b}$ is a consistent or inconsistent system.

(c) &emsp; Hence or otherwise, solve $A \mathbf{x} = \mathbf{b}$.

```{dropdown} Solution
(a) 

$$ \begin{align*}
    \det(A) &= \begin{vmatrix} 0 & -1 & 5 \\ 8 & 1 & 2 \\ 5 & 2 & -1 \end{vmatrix}
    = \begin{vmatrix} 8 & 2 \\ 5 & -1 \end{vmatrix} + 5\begin{vmatrix} 8 & 1 \\ 5 & 2 \end{vmatrix} = -18 + 55 = 37, \\
    \operatorname{adj}(A) &= \begin{pmatrix} -5 & 18 & 11 \\ 9 & -25 & -5 \\ -7 & 40 & 8 \end{pmatrix}^\mathsf{T} 
    = \begin{pmatrix} -5 & 9 & -7 \\ 18 & -25 & 40 \\ 11 & -5 & 8 \end{pmatrix}, \\
    A^{-1} &= \frac{\operatorname{adj}(A)}{\det(A)} = \frac{1}{37} \begin{pmatrix} -5 & 9 & -7 \\ 18 & -25 & 40 \\ 11 & -5 & 8 \end{pmatrix}.           
\end{align*} $$

To show the inverse is correct we use $A^{-1}A = I$

$$ \begin{align*}
    \frac{1}{37} \begin{pmatrix} -5 & 9 & -7 \\ 18 & -25 & 40 \\ 11 & -5 & 8 \end{pmatrix}
    \begin{pmatrix} 0 & -1 & 5 \\ 8 & 1 & 2 \\ 5 & 2 & -1 \end{pmatrix} =
    \frac{1}{37} \begin{pmatrix} 37 & 0 \\ 0 & 37 \\ 0 & 0 & 37 \end{pmatrix} =
    \begin{pmatrix} 1 & 0 \\ 0 & 1 \\ 0 & 0 & 1 \end{pmatrix}.
\end{align*} $$

(b)

$$\begin{align*}
    & \begin{pmatrix}
        0 & -1 & 5 & 2 \\
        8 & 1 & 2 & 1 \\
        5 & 2 & -1 & 0 
   \end{pmatrix}
    \begin{array}{l} R_1 \leftrightarrow R_2 \\ \phantom{x} \\ \phantom{x} \end{array} 
    & \longrightarrow
    & \begin{pmatrix}
        8 & 1 & 2 & 1 \\
        0 & -1 & 5 & 2 \\
        5 & 2 & -1 & 0 
   \end{pmatrix}
    \begin{array}{l}  \\ \\ R_3 - \frac{5}{8} R_1 \end{array} \\
    \longrightarrow
    & \begin{pmatrix}
        8 & 1 & 2 & 1 \\
        0 & -1 & 5 & 2 \\
        0 & \frac{11}{8} & -\frac{9}{4} & -\frac{5}{8}
   \end{pmatrix}
    \begin{array}{l}  \\ \\ R_3 + \frac{11}{8}R_2 \end{array} 
    & \longrightarrow
    & \begin{pmatrix}
        8 & 1 & 2 & 1 \\
        0 & -1 & 5 & 2 \\
        0 & 0 & \frac{37}{8} & \frac{17}{8}
   \end{pmatrix} 
\end{align*} $$

$\operatorname{rank}(A) = \operatorname{rank}([A \mid \mathbf{b}]) = 3$ so the system $A \mathbf{x} = \mathbf{b}$ is a consistent system. 

(c)

Using back substitution on the row echelon form of $(A \mid \mathbf{b})$

$$ \begin{align*}
    x_3 &= \frac{8}{37}\left(\frac{17}{8}\right) = \frac{17}{37}, \\
    x_2 &= -\left(2 - 5 \left( \frac{17}{37}\right) \right) = \frac{11}{37}, \\
    x_1 &= \frac{1}{8} \left(1 - \frac{11}{37} - 2\left(\frac{17}{37}\right)\right) = -\frac{1}{37}.
\end{align*} $$
```

---

2\. Two lines $\ell_1$ and $\ell_2$ in $\mathbb{R}^3$ are defined using

$$ \begin{align*}
    \ell_1: \begin{pmatrix} 0 \\ -2 \\ 6 \end{pmatrix} + t_1 \begin{pmatrix} -1 \\ 2 \\ 0 \end{pmatrix}, \\
    \ell_2: \begin{pmatrix} 0 \\ 3 \\ -2 \end{pmatrix} + t_2 \begin{pmatrix} -1 \\ 2 \\ 1 \end{pmatrix},
\end{align*} $$

where $t \in \mathbb{R}$.

(a) &emsp; Determine whether the lines intersect and if so, state where.

(b) &emsp; Find the shortest distance from the point $(0, 0, 1)$ to the line $\ell_1$.

(c) &emsp; Find the equation of the plane containing the points $(4, 1, 1)$, $(2, 1, 0)$ and $(1, 3, 4)$.

(d) &emsp; Does the point with co-ordinates $(0, -1, 1)$ lie on the plane as the points with co-ordinates $(4, 1, 1)$, $(2, 1, 0)$ and $(1, 3, 4)$? Justify your answer.

```{dropdown} Solution
(a) &emsp; Equating $\ell_1$ and $\ell_2$

$$ \begin{align*}
    -t_1 &= -t_2, \\
    -2 + 2t_1 &= 3 + 2t_2, \\
    6 &= -2 + t_1.
\end{align*} $$

The third equation gives $t_1 = 8$ which substituted into the first equation gives $t_2 = 8$. Substituting both of these into the second equations gives $-2+2(8) \neq 3 + 2(8)$ so $\ell_1$ and $\ell_2$ do not intersect.

(b) &emsp; Using $t = \dfrac{(\mathbf{q} - \mathbf{p}) \cdot \mathbf{d}}{ \mathbf{d} \cdot \mathbf{d}}$ where $\mathbf{q} = (0, 0, 1)$, $\mathbf{p} = (0, -2, 6)$ and $\mathbf{d} = (-1, 2, 0)$ gives

$$ \begin{align*}
    t &= \frac{((0,0,1) - (0, -2, 6)) \cdot (-1, 2, 0)}{(-1, 2, 0) \cdot (-1, 2, 0)}
    = \frac{4}{5}.
\end{align*}$$

Therefore the point on the line $\ell_1$ closest to $(0, 0, 1)$ is

$$ \begin{align*}
    \mathbf{r} = (0, -2, 6) + \frac{4}{5}(1, 2, 0) = \left( -\frac{4}{5}, -\frac{2}{5}, 6 \right),
\end{align*} $$

so the shortest distance from $(0, 0, 1)$ to the line $\ell_1$ is

$$ \begin{align*}
    d &= \left\| \left( -\frac{4}{5}, -\frac{2}{5}, 6 \right)  - (0, 0, 1) \right\|
    = \sqrt{\left(-\frac{4}{5}\right)^2 + \left(-\frac{2}{5}\right)^2 + 5^2} \\
    &= \frac{\sqrt{645}}{5}
    \approx 5.0794.
\end{align*} $$

(c) &emsp; Calculate the normal to the plane

$$ \begin{align*}
    \mathbf{n} &= ((2, 1, 0) - (4, 1, 1)) \times ((1, 3, 4) - (4, 1, 1))
    = (-2, 0, -1) \times (-3, 2, 3) \\
    &= \begin{vmatrix} \mathbf{i} & \mathbf{j} & \mathbf{k} \\ -2 & 0 & -1 \\ -3 & 2 & 3 \end{vmatrix} = (2, 9, -4).
\end{align*} $$

Using the point-normal equation of a plane

$$ \begin{align*}
    \mathbf{n} \cdot (x - x_0, y - y_0, z - z_0) &= 0 \\
    (2, 9, -4) \cdot (x - 2, y - 1, z - 0) &= 0 \\
    2x + 9y - 4z - 13 &= 0.
\end{align*} $$

(d) &emsp; Substituting $x = 0$, $y = -1$ and $z = 1$ into the equation of the plane from part (b)

$$ \begin{align*}
    2(0) + 9(-1) - 4(1) - 13 &= 0,
\end{align*} $$

therefore, $(0, -1, 1)$ does lie on the same plane as $(4, 1, 1)$, $(2, 1, 0)$ and $(1, 3, 4)$.
```

---

3\. (a) &emsp; Vectors in $\mathbb{R}^3$ are defined by $\mathbf{a} = (3, -1, 12)$ and $\mathbf{b} = (4, 2, 3)$.

&emsp; (i) &emsp; Determine $4\mathbf{a} - 6\mathbf{b}$.

&emsp; (ii) &emsp; Calculate $\mathbf{a} \cdot \mathbf{b}$.

&emsp; (iii) &emsp; Find the length of the vector $3 \mathbf{a} - \mathbf{b}$.

&emsp; (iv) &emsp; Determine $\mathbf{a} \times (\mathbf{a} \times \mathbf{b})$.

&emsp; (v) &emsp; Show that the following set of vectors form a basis for $\mathbb{R}^3$.

(b) &emsp; Show that the following set of vectors form a basis for $\mathbb{R}^3$

$$ \begin{align*}
    B = \left\{ \begin{pmatrix} 1 \\ 2 \\ 3 \end{pmatrix},
    \begin{pmatrix} 1 \\ 0 \\ 1 \end{pmatrix},
    \begin{pmatrix} 1 \\ -1 \\ 5 \end{pmatrix} \right\}.
\end{align*} $$

(c) &emsp; Determine the change of basis matrix $A_{E\to B}$ such that

$$A_{E\to B} [\mathbf{u}]_E= [\mathbf{u}]_B,$$

where $E= \{ \mathbf{e}_1, \mathbf{e}_2, \mathbf{e}_3 \}$ is the standard basis. Uses your matrix to express the vector $[(2, 2, 1)]_E$ with respect to the basis $B$ from part (b).

```{dropdown} Solution
(a) (i)

$$\begin{align*}
    4 \mathbf{a} - 6 \mathbf{b}
    = 4( 3, -1, 12) - 6 (4, 2, 3)
    = (12, -4, 48) - (24, 12, 18)
    = (-12, -16, 30).
\end{align*}$$

(a) (ii)

$$\begin{align*}
    \mathbf{a} \cdot \mathbf{b} = (3, -1, 12) \cdot (4, 2, 3)
    = 12 - 2 + 36 = 46.
\end{align*}$$

(a) (iii)

$$\begin{align*}
    \|3 \mathbf{a} - \mathbf{b}\| &= \| 3 (3, -1, 12) - (4, 2, 3) \|
    = \| (5, -5, 33) \| \\
    &= \sqrt{5^2 + (-5)^2 + 33^2} = \sqrt{1139} \approx 33.7491.
\end{align*}$$

(a) (iv)

$$\begin{align*}
    \mathbf{a} \times (\mathbf{a} \times \mathbf{b}) &=
    (3, -1, 12) \times ((3, -1, 12) \times (4, 2, 3)) \\
    &= (3, -1, 12) \times \begin{vmatrix} \mathbf{i} & \mathbf{j} & \mathbf{k} \\ 3 & -1 & 12 \\ 4 & 2 & 3 \end{vmatrix}
    = (3, -1, 12) \times (-27, 39, 10) \\
    &= \begin{vmatrix} \mathbf{i} & \mathbf{j} & \mathbf{k} \\ 3 & -1 & 12 \\ -27 & 39 & 10 \end{vmatrix}
    = (-478, -354, 90).
\end{align*}$$

(b) &emsp; We need to show the vectors are linearly independent

$$\begin{align*}
    && \begin{pmatrix}
        1 & 1 & 1 \\
        2 & 0 & -1 \\
        3 & 1 & 5
   \end{pmatrix}
    \begin{array}{l} \\ R_2 - 2R_1 \\ R_3 - 3 R_1 \end{array} &
    & \longrightarrow
    & \begin{pmatrix}
        1 & 1 & 1 \\
        0 & -1 & -3 \\
        0 & -2 & 2
   \end{pmatrix}
    \begin{array}{l} \\ -R_2 \\ \phantom{x} \end{array} \\ \\
    & \longrightarrow
    & \begin{pmatrix}
        1 & 1 & 1 \\
        0 & 1 & 3 \\
        0 & -2 & 2
   \end{pmatrix}
    \begin{array}{l} R_1 - R_2 \\ \\ R_3 + 2R_1 \end{array} &
    & \longrightarrow
    & \begin{pmatrix}
        1 & 0 & -2 \\
        0 & 1 & 3 \\
        0 & 0 & -1
   \end{pmatrix}
    \begin{array}{l}  \\ \\ - R_3 \end{array} \\ \\
    & \longrightarrow
    & \begin{pmatrix}
        1 & 0 & -2 \\
        0 & 1 & 3 \\
        0 & 0 & 1
   \end{pmatrix}
    \begin{array}{l} R_1 + 2R_3 \\ R_2 - 3R_3\\  \phantom{x}\end{array} &
    & \longrightarrow
    & \begin{pmatrix}
        1 & 0 & 0 \\
        0 & 1 & 0 \\
        0 & 0 & 1
   \end{pmatrix}
\end{align*}$$

So the vectors in $B$ are linearly independent. They also span $\mathbb{R}^3$ since the rank of the matrix formed by the three vectors is 3, therefore $B$ is a basis for $\mathbb{R}^3$.

(c) &emsp; Since $A_{E\to B} [\mathbf{u}]_E= [\mathbf{u}]_B$ then $A_{E\to B}$ is the inverse of the matrix formed from the vectors in $B$.

$$\begin{align*}
    \det \begin{pmatrix} 1 & 1 & 1 \\ 2 & 0 & -1 \\ 3 & 1 & 5 \end{pmatrix} &=
    -13 + 3 = -10, \\
    \operatorname{adj} \begin{pmatrix} 1 & 1 & 1 \\ 2 & 0 & -1 \\ 3 & 1 & 5 \end{pmatrix} &=
    \begin{pmatrix} 1 & -13 & 2 \\ -4 & 2 & 2 \\ -1 & 3 & -2 \end{pmatrix}^\mathsf{T} =
    \begin{pmatrix} 1 & -4 & -1 \\ -13 & 2 & 3 \\ 2 & 2 & -2 \end{pmatrix}, \\
    \therefore A_{E \to B} &= \frac{1}{-10} \begin{pmatrix} 1 & -4 & -1 \\ -13 & 2 & 3 \\ 2 & 2 & -2 \end{pmatrix} \\
    &= \frac{1}{10} \begin{pmatrix} -1 & 4 & 1 \\ 13 & -2 & -3 \\ -2 & -2 & 2 \end{pmatrix}.
\end{align*}$$

Determining $[(2, 2, 1)]_B$

$$\begin{align*}
    \left[ \begin{pmatrix} 2 \\ 2 \\ 1 \end{pmatrix} \right]_B &=
    \frac{1}{10} \begin{pmatrix} -1 & 4 & 1 \\ 13 & -2 & -3 \\ -2 & -2 & 2 \end{pmatrix}
    \begin{pmatrix} 2 \\ 2 \\ 1 \end{pmatrix} =
    \frac{1}{10} \begin{pmatrix} 7 \\ 19 \\ -6 \end{pmatrix} =
    \begin{pmatrix} \frac{7}{10} \\[2pt] \frac{19}{10} \\[2pt] -\frac{3}{5} \end{pmatrix}.
\end{align*}$$
```

---

4\. (a) &emsp; Determine which of the following subsets of the vector space of $M_{2}(\mathbb{R})$ (the space of all $2\times 2$ matrices) are subspaces over $\mathbb{R}$:

&emsp; (i) &emsp; $W_1 = \left\{ \begin{pmatrix} a & b \\ c & d \end{pmatrix} : a - b = c - d \right\}$;

&emsp; (ii) &emsp; $W_2 = \left\{ \begin{pmatrix} a & b \\ c & d \end{pmatrix} : ab = cd \right\}$.

(b) &emsp; Show that the vectors

$$\begin{align*}
    \left\{ \begin{pmatrix} a & b \\ b & 0 \end{pmatrix}, \begin{pmatrix} a - b & b \\ c & 0 \end{pmatrix}, \begin{pmatrix} 4b - 2a & -2b \\ 2b - 4c & 0 \end{pmatrix} \right\} \subset M_{2}(\mathbb{R}),
\end{align*}$$

are linearly dependent over $\mathbb{R}$.

(c) &emsp; Determine the co-ordinates of the vector $A = \begin{pmatrix} 2 & 1 \\ 4 & -1 \end{pmatrix}$ with respect to the basis

$$ \begin{align*}
    B = \left\{ \begin{pmatrix} 1 & 1 \\ 0 & 0 \end{pmatrix} ,
    \begin{pmatrix} 1 & 0 \\ 2 & 1 \end{pmatrix},
    \begin{pmatrix} 0 & 0 \\ 1 & -1 \end{pmatrix} \right\}.
\end{align*} $$

```{dropdown} Solution
(a) (i) &emsp; Let $U = \begin{pmatrix} u_{11} & u_{12} \\ u_{11} - u_{12} & 0 \end{pmatrix}, V = \begin{pmatrix} v_{11} & v_{12} \\ v_{11} - v_{12} & 0 \end{pmatrix} \in W_1$ and $\alpha \in \mathbb{R}$ then $W_1$ is a subspace if $U + \alpha V \in W_1$.

$$\begin{align*}
    U + \alpha V &=
    \begin{pmatrix} u_{11} & u_{12} \\ u_{11} - u_{12} & 0 \end{pmatrix} + \alpha
    \begin{pmatrix} v_{11} & v_{12} \\ v_{11} - v_{12} & 0 \end{pmatrix} \\
    &=
    \begin{pmatrix} u_{11} + \alpha v_{11} & u_{12} + \alpha v_{11}  \\ u_{11} - u_{12} + \alpha(v_{11} - v_{12}) & 0 \end{pmatrix} \in W_1
\end{align*}$$

so $W_1$ is a subspace of $M_{2}(\mathbb{R})$.

(a) (ii) &emsp; $W_2$ is not a subspace since for $U = \begin{pmatrix} 1 & 1 \\ 2 & \frac{1}{2} \end{pmatrix}, V = \begin{pmatrix} 1 & 3 \\ 9 & \frac{1}{3} \end{pmatrix} \in W_2$ we have

$$\begin{align*}
    V + W &= \begin{pmatrix} 1 & 1 \\ 2 & \frac{1}{2} \end{pmatrix} +
    \begin{pmatrix} 1 & 3 \\ 9 & \frac{1}{3} \end{pmatrix}
    = \begin{pmatrix} 2 & 4 \\ 11 & \frac{5}{6} \end{pmatrix},
\end{align*}$$

which is not in $W_2$ because $2 \times 4 = 8 \neq 11 \times \frac{5}{6} = \frac{55}{6}$.

(b) &emsp; We need to show that

$$\begin{align*}
    \alpha_1 \begin{pmatrix} a & b \\ b & 0 \end{pmatrix} + \alpha_2
    \begin{pmatrix} a - b & b \\ c & 0 \end{pmatrix} + \alpha_3
    \begin{pmatrix} 4b - 2a & -2b \\ 2b - 4c & 0 \end{pmatrix} &= \mathbf{0},
\end{align*}$$

and ignoring the element in row 2 column 2 of each matrix and reshaping them into $3 \times 1$ vectors we have

$$\begin{align*}
    \alpha_1 \begin{pmatrix} a \\ b \\ b \end{pmatrix} + \alpha_2
    \begin{pmatrix} a-b \\ b \\ c \end{pmatrix} + \alpha_3
    \begin{pmatrix} 4b - 2a \\ -2b \\ 2b - 4a \end{pmatrix} &=
    \begin{pmatrix} 0 \\ 0 \\ 0 \end{pmatrix}.
\end{align*}$$

Using Gauss-Jordan elimination to solve for $\alpha_1$, $\alpha_2$ and $\alpha_3$

$$\begin{align*}
    & \begin{pmatrix}
        a & a - b & 4b - 2a \\
        b & b & -2b \\
        b & c & 2b - 4c
    \end{pmatrix}
    \begin{array}{l} R_1 \leftrightarrow R_2 \\ \phantom{x} \\ \phantom{x} \end{array} &
    \longrightarrow
    & \begin{pmatrix}
        b & b & -2b \\
        a & a - b & 4b - 2a \\
        b & c & 2b - 4c
    \end{pmatrix}
    \begin{array}{l} \frac{1}{b}R_1 \\ \phantom{x} \\ \phantom{x} \end{array} \\ \\
    \longrightarrow
    & \begin{pmatrix}
        1 & 1 & -2 \\
        a & a - b & 4b - 2a \\
        b & c & 2b - 4c
    \end{pmatrix}
    \begin{array}{l}  \\ R_2 - aR_1 \\ R_3 - bR_1 \end{array} &
    \longrightarrow
    & \begin{pmatrix}
        1 & 1 & -2 \\
        0 & - b & 4b \\
        0 & c - b & 4b - 4c
    \end{pmatrix}
    \begin{array}{l}  \\ -\frac{1}{b}R_2 \\ \phantom{x} \end{array} \\ \\
    \longrightarrow
    & \begin{pmatrix}
        1 & 1 & -2 \\
        0 & 1 & -4 \\
        0 & c - b & 4b - 4c
    \end{pmatrix}
    \begin{array}{l}  R_1 - R_2 \\ \\R_3 - (c - b)R_2 \end{array} &
    \longrightarrow
    & \begin{pmatrix}
        1 & 0 & 2 \\
        0 & 1 & -4 \\
        0 & 0 & 0
    \end{pmatrix}
\end{align*}$$

Let $\alpha_3 = s$ then $\alpha_2 = 4s$ and $\alpha_1 = -2s$. Since we have non-zero solutions then the three vectors are linearly dependant.

(c) &emsp; We need to solve the equation

$$\begin{align*}
    \alpha_1 \begin{pmatrix} 1 & 1 \\ 0 & 0 \end{pmatrix} + \alpha_2
    \begin{pmatrix} 1 & 0 \\ 2 & 1 \end{pmatrix} + \alpha_3
    \begin{pmatrix} 0 & 0 \\ 1 & -1 \end{pmatrix}
    = \begin{pmatrix} 2 & 1 \\ 4 & - 1\end{pmatrix}.
\end{align*}$$

We can reshape the matrices into $4\times 1$ vectors so that

$$\begin{align*}
    \alpha_1
    \begin{pmatrix} 1 \\ 1 \\ 0 \\ 0 \end{pmatrix} + \alpha_2
    \begin{pmatrix} 1 \\ 0 \\ 2 \\ 1 \end{pmatrix} + \alpha_3
    \begin{pmatrix} 0 \\ 0 \\ 1 \\ -1 \end{pmatrix} &=
    \begin{pmatrix} 2 \\ 1 \\ 4 \\ -1 \end{pmatrix}.
\end{align*}$$

Using Gauss-Jordan elimination:

$$\begin{align*}
    & \left( \begin{array}{ccc|c}
        1 & 0 & 0 & 1 \\
        1 & 1 & 0 & 2 \\
        0 & 2 & 1 & 4 \\
        0 & 1 & -1 & -1
    \end{array} \right)
    \begin{array}{l} \\ R_2 - R_1 \\ \phantom{x} \\ \phantom{x}  \end{array} &
    \longrightarrow
    & \left( \begin{array}{ccc|c}
        1 & 0 & 0 & 1 \\
        0 & 1 & 0 & 1 \\
        0 & 2 & 1 & 4 \\
        0 & 1 & -1 & -1
    \end{array} \right)
    \begin{array}{l} \phantom{x} \\ \phantom{x} \\ R_3 - 2R_2 \\ R_4 - R_2 \end{array} \\
    \longrightarrow
    & \left( \begin{array}{ccc|c}
        1 & 0 & 0 & 1 \\
        0 & 1 & 0 & 1 \\
        0 & 0 & 1 & 2 \\
        0 & 0 & -1 & -2
    \end{array} \right)
    \begin{array}{l} \phantom{x} \\  \phantom{x} \\  \phantom{x} \\ R_4 + R_3 \end{array} &
    \longrightarrow
    & \left( \begin{array}{ccc|c}
        1 & 0 & 0 & 1 \\
        0 & 1 & 0 & 1 \\
        0 & 0 & 1 & 2 \\
        0 & 0 & 0 & 0
    \end{array} \right)
\end{align*}$$

So $[A]_B = (1, 1, 2)$.
```

---

5\. &emsp; Let $P_3(\mathbb{R})$ denote a vector space of all polynomials of degree at most three with real coefficients. Given the mapping $M_2(\mathbb{R}) \to P_3(\mathbb{R})$ defined by

$$\begin{align*}
    T \begin{pmatrix} a & b \\ c & d \end{pmatrix} = (a + b) + (c - d)x^3.
\end{align*}$$

(a) &emsp; Determine $T\begin{pmatrix} -1 & 2 \\ 0 & 3 \end{pmatrix}$.

(b) &emsp; Determine non-zero vectors $A, B \in M_{2}(\mathbb{R})$ such that $T(A) = 5 + x^3$ and $T(B) = 0$.

(c) &emsp; Given that $U = \begin{pmatrix} 9 & 1 \\ -1 & 0 \end{pmatrix}$ determine $T(3U)$.

(d) &emsp; Prove that $T$ is a linear transformation.

```{dropdown} Solution

(a) &emsp; $T\begin{pmatrix} -1 & 2 \\ 0 & 3 \end{pmatrix} = (-1 + 2) + (0 - 3)x^3 = 1 - 3x^3.$

(b) &emsp; For $A$ we need

$$\begin{align*}
    a + b &= 5, \\
    c - d &= 1
\end{align*}$$

so let $a = 5$, $b = 0$, $c = 1$ and $d = 0$ then $A = \begin{pmatrix} 5 & 0 \\ 1 & 0 \end{pmatrix}$.

For $B$ we need

$$\begin{align*}
    a + b &= 0, \\
    c - d &= 0
\end{align*}$$

so let $a = 1$, $b = -1$, $c = 1$ and $d = 1$ then $B = \begin{pmatrix} 1 & -1 \\ 1 & 1 \end{pmatrix}$.

(c) &emsp; $T\left(3 \begin{pmatrix} 9 & 1 \\ -1 & 0 \end{pmatrix} \right) = T \begin{pmatrix} 27 & 3 \\ -3 & 0 \end{pmatrix} = 30 - 3 x^3.$

(d) &emsp; $T$ is a linear transformation if $T(\mathbf{u} + \alpha \mathbf{v}) = T(\mathbf{u}) + \alpha T(\mathbf{v})$. Let $U = \begin{pmatrix} u_{11} & u_{12} \\ u_{21} & u_{22} \end{pmatrix}$ and $V = \begin{pmatrix} v_{11} & v_{12} \\ v_{21} & v_{22} \end{pmatrix}$

$$\begin{align*}
    T(U + \alpha V) &= T\left(  \begin{pmatrix} u_{11} & u_{12} \\ u_{21} & u_{22} \end{pmatrix} + \alpha
    \begin{pmatrix} v_{11} & v_{12} \\ v_{21} & v_{22} \end{pmatrix} \right) \\
    &= T\begin{pmatrix} u_{11} + \alpha v_{11} & u_{12} + \alpha v_{12} \\ u_{21} + \alpha v_{21} & u_{22} + \alpha v_{22} \end{pmatrix} \\
    &= (u_{11} + \alpha v_{11} + u_{12} + \alpha v_{12}) + (u_{21} + \alpha v_{21} - u_{22} - \alpha v_{22})x^3, \\
    T(U) + \alpha T(V) &= T \begin{pmatrix} u_{11} & u_{12} \\ u_{21} & u_{22} \end{pmatrix} + \alpha T
    \begin{pmatrix} v_{11} & v_{12} \\ v_{21} & v_{22} \end{pmatrix} \\
    &= (u_{11} + u_{12}) + (u_{21} - u_{22})x^3  + \alpha (v_{11} + v_{12}) + \alpha (v_{21} - v_{22}) x^3 \\
    &= (u_{11} + \alpha v_{11} + u_{12} + \alpha v_{12}) + (u_{21} + \alpha v_{21} - u_{22} - \alpha v_{22}) x^3.
\end{align*}$$

Therefore, $T$ is a linear transformation.
```
